deps/poulet4/lib/P4cub/BigStep/Value/Auxilary.v
@@ -4,28 +4,17 @@ Import Val ValueNotations P.P4cubNotations.
 
 (** Intial/Default value from a type. *)
 Fixpoint vdefault (τ : E.t) : v :=
-  let fix lstruct (ts : list E.t) : list v :=
-      match ts with
-      | [] => []
-      | τ :: ts => vdefault τ :: lstruct ts
-      end in
-  let fix fields_struct
-          (ts : F.fs string E.t) : F.fs string v :=
-      match ts with
-      | [] => []
-      | (x, τ) :: ts => (x, vdefault τ) :: fields_struct ts
-      end in
   match τ with
-  | {{ error }}      => VError None
-  | {{ matchkind }}  => VMatchKind E.MKExact
-  | {{ Bool }}       => VBool false
+  | {{ error }}      => ~{ ERROR None }~
+  | {{ matchkind }}  => ~{ MATCHKIND exact }~
+  | {{ Bool }}       => ~{ FALSE }~
   | {{ bit<w> }}     => VBit w 0%Z
   | {{ int<w> }}     => VInt w 0%Z
-  | {{ tuple ts }}   => VTuple (lstruct ts)
-  | {{ struct { ts } }} => VStruct (fields_struct ts)
-  | {{ hdr { ts } }} => VHeader (fields_struct ts) false
+  | {{ tuple ts }}   => VTuple $ List.map vdefault ts
+  | {{ struct { ts } }} => VStruct $ F.map vdefault ts
+  | {{ hdr { ts } }} => VHeader (F.map vdefault ts) false
   | {{ stack fs[n] }} => VHeaderStack
-                          fs (repeat (false, fields_struct fs)
+                          fs (repeat (false, F.map vdefault fs)
                                      (Pos.to_nat n)) n 0
   end.
 (**[]*)
@@ -52,40 +41,52 @@ Fixpoint match_pattern (p : PR.pat) (V : v) : bool :=
   end.
 (**[]*)
 
+Fixpoint approx_type (V : v) : E.t :=
+  match V with
+  | ~{ VBOOL _ }~ => {{ Bool }}
+  | ~{ w VW _ }~ => {{ bit<w> }}
+  | ~{ w VS _ }~ => {{ int<w> }}
+  | ~{ ERROR _ }~ => {{ error }}
+  | ~{ MATCHKIND _ }~ => {{ matchkind }}
+  | ~{ TUPLE vs }~ => E.TTuple $ List.map approx_type vs
+  | ~{ STRUCT { vs } }~
+    => E.TStruct $ F.map approx_type vs
+  | ~{ HDR { vs } VALID:=_ }~
+    => E.THeader $ F.map approx_type vs
+  | ~{ STACK _:ts[n] NEXT:=_ }~ => {{ stack ts[n] }}
+  end.
+(**[]*)
+                      
 Section Util.
   Context {tags_t : Type}.
   
-  (* TODO: uhhh... *)
-  Fail Fixpoint expr_of_value (i : tags_t) (V : v) : E.e tags_t :=
-    let fix lstruct (vs : list v) : list (E.e tags_t) :=
-        match vs with
-        | []      => []
-        | hv :: tv => expr_of_value i hv :: lstruct tv
-        end in
-    let fix fstruct (vs : F.fs string v)
-        : F.fs string (E.t * E.e tags_t) :=
-        match vs with
-        | [] => []
-        | (x, hv) :: vs => (x, (_, expr_of_value i hv)) :: fstruct vs (* TODO *)
-        end in
-    let fix stkstruct (hs : list (bool * F.fs string v))
-        : list (E.e tags_t) :=
-        match hs with
-        | [] => []
-        | (b, vs) :: hs
-          => E.EHeader (fstruct vs) <{ BOOL b @ i }> i :: stkstruct hs
-        end in
+  Fixpoint expr_of_value (i : tags_t) (V : v) : E.e tags_t :=
     match V with
     | ~{ VBOOL b }~ => <{ BOOL b @ i }>
     | ~{ w VW n }~ => <{ w W n @ i }>
     | ~{ w VS z }~ => <{ w S z @ i }>
     | ~{ ERROR err }~ => <{ Error err @ i }>
     | ~{ MATCHKIND mk }~ => <{ Matchkind mk @ i }>
-    | ~{ TUPLE vs }~ => E.ETuple (lstruct vs) i
-    | ~{ STRUCT { vs } }~ => E.EStruct (fstruct vs) i
+    | ~{ TUPLE vs }~
+      => E.ETuple (List.map (expr_of_value i) vs) i
+    | ~{ STRUCT { vs } }~
+      => E.EStruct
+          (F.map
+             (fun v => (approx_type v, expr_of_value i v))
+             vs) i
     | ~{ HDR { vs } VALID:=b }~
-      => E.EHeader (fstruct vs) <{ BOOL b @ i }> i
-    | ~{ STACK vs:ts[n] NEXT:=ni }~
-      => E.EHeaderStack ts (stkstruct vs) n ni
+      => E.EHeader
+          (F.map
+             (fun v => (approx_type v, expr_of_value i v))
+             vs) <{ BOOL b @ i }> i
+    | ~{ STACK hs:ts[n] NEXT:=ni }~
+      => E.EHeaderStack
+          ts
+          (List.map
+             (fun '(b,vs) =>
+                E.EHeader
+                  (F.map
+                     (fun v => (approx_type v, expr_of_value i v))
+                     vs) <{ BOOL b @ i }> i) hs) n ni i
     end.
 End Util.
