deps/poulet4/lib/P4cub/Static/Auxilary.v
@@ -1,0 +1,19 @@
+Set Warnings "-custom-entry-overridden".
+Require Import
+        Poulet4.P4cub.Envn
+        Poulet4.P4cub.Syntax.Syntax
+        Poulet4.P4cub.Static.Util
+        Poulet4.P4cub.Static.Typing
+        Poulet4.P4cub.Static.IndPrincip.
+Import P.P4cubNotations.
+
+(** TODO *)
+Section TypeOf.
+  Context {tags_t : Type}.
+  
+  Fail Fixpoint type_of_expr (Γ : gamma) (e : E.e tags_t) : option E.t :=
+    match e with
+    | <{ BOOL _ @ _ }> => Some {{ Bool }}
+    | <{ w W n @ _ }> => None
+    end.
+End TypeOf.
